Weidenbach_Book/IsaSAT/IsaSAT_Initialisation.thy
@@ -2141,9 +2141,9 @@ lemma finalise_init_finalise_init_full:
   apply (cases S; cases T)
   apply (simp add: finalise_init_code_def)
   apply (auto simp: finalise_init_def twl_st_heur_def twl_st_heur_parsing_no_WL_def
-    twl_st_heur_parsing_no_WL_wl_def
+    twl_st_heur_parsing_no_WL_wl_def distinct_mset_dom
       finalise_init_code_def out_learned_def all_lits_st_alt_def[symmetric]
-      twl_st_heur_post_parsing_wl_def all_atms_st_def ac_simps
+      twl_st_heur_post_parsing_wl_def all_atms_st_def ac_simps aivdom_inv_def
     intro!: ASSERT_leI intro!: isa_vmtf_init_isa_vmtf heuristic_rel_initI
     dest: isa_vmtf_init_nemptyD)
   done
